Add simple addition extraction test

code/experimental/he/Hacl.Impl.HE.GM.fst
@@ -10,10 +10,8 @@ open Lib.IntTypes
 open Lib.Buffer
 open Lib.PrintBuffer
 
-module S = Hacl.Spec.HE.GM
+open Hacl.Impl.Addition
+open Hacl.Impl.Lib
 
-inline_for_extraction noextract
-let lbytes (len : size_t) = lbuffer uint8 len
-
-inline_for_extraction noextract
-let lbignum (len : size_t) = lbuffer uint64 len
+val testfunc : lbytes 5ul -> lbytes 6ul
+let testfunc _ = admit()
